Update to branch robbert/local_updates of Iris.
Main changes:

- Use new notion of local updates.
- Use new big operators over CMRAs.
- Factor out common properties of lrust in heap.

adequacy.v
@@ -1,22 +1,33 @@
 From iris.program_logic Require Export weakestpre adequacy.
 From lrust Require Export heap.
-From iris.program_logic Require Import auth ownership.
+From iris.algebra Require Import auth.
+From iris.program_logic Require Import ownership.
 From lrust Require Import proofmode notation.
 From iris.proofmode Require Import tactics weakestpre.
 From iris.prelude Require Import fin_maps.
 
-Definition heap_adequacy Σ `{irisPreG lrust_lang Σ, authG Σ heapValUR, authG Σ heapFreeableUR} e σ φ :
+Class heapPreG Σ := HeapPreG {
+  heap_preG_iris :> irisPreG lrust_lang Σ;
+  heap_preG_heap :> inG Σ (authR heapUR);
+  heap_preG_heap_freeable :> inG Σ (authR heap_freeableUR)
+}.
+
+Definition heapΣ : gFunctors :=
+  #[irisΣ lrust_lang;
+    GFunctor (constRF (authR heapUR));
+    GFunctor (constRF (authR heap_freeableUR))].
+Instance subG_heapPreG {Σ} : subG heapΣ Σ → heapPreG Σ.
+Proof. intros [? [?%subG_inG ?%subG_inG]%subG_inv]%subG_inv. split; apply _. Qed.
+
+Definition heap_adequacy Σ `{heapPreG Σ} e σ φ :
   (∀ `{heapG Σ}, heap_ctx ⊢ WP e {{ v, ■ φ v }}) →
   adequate e σ φ.
 Proof.
-  intros Hwp; eapply (wp_adequacy Σ); iIntros (?) "Hσ".
-  iVs (own_alloc (● to_heapVal σ)) as (vγ) "Hvγ".
-  { split; last apply to_heap_valid. intro. simpl. refine (ucmra_unit_leastN _ _). }
-  iVs (own_alloc (● (∅ : heapFreeableUR))) as (fγ) "Hfγ".
-  { split. intro. refine (ucmra_unit_leastN _ _). exact ucmra_unit_valid. }
-  set (h:=HeapG _ _ _ _ vγ fγ).
-  iVs (inv_alloc heapN _ heap_inv with "[-]") as "HN";
-    last by iApply (Hwp h); rewrite /heap_ctx.
-  iNext. iExists _, _. iFrame. iPureIntro. intros ??. rewrite lookup_empty.
-  inversion 1.
+  intros Hwp; eapply (wp_adequacy Σ). iIntros (?) "Hσ".
+  iVs (own_alloc (● to_heap σ)) as (vγ) "Hvγ".
+  { apply (auth_auth_valid (to_heap _)), to_heap_valid. }
+  iVs (own_alloc (● (∅ : heap_freeableUR))) as (fγ) "Hfγ"; first done.
+  set (Hheap := HeapG _ _ _ _ vγ fγ).
+  iVs (inv_alloc heapN _ heap_inv with "[-]"); [iNext; iExists σ, ∅; by iFrame|].
+  iApply (Hwp _). by rewrite /heap_ctx.
 Qed.
